theories/prob_eff_lang/probblaze/examples/DH_KE/dhke_channel.v
@@ -8,12 +8,12 @@ From clutch.prob_eff_lang.probblaze Require Import logic primitive_laws proofmod
   class_instances. 
 From clutch.prob_eff_lang.probblaze Require Import tactics.
 From clutch.prob_eff_lang.probblaze Require Import def_dhke.
+From clutch.prob_eff_lang.probblaze Require Import sem_types sem_row sem_sig sem_judgement sem_def. 
 
 Import fingroup.
 
 Import fingroup.fingroup.
 
-Import valgroup_notation.
 Import valgroup_tactics.
 
 Section handlee_verification.
@@ -122,6 +122,17 @@ Section handlee_verification.
 
   Definition T : iThy Σ := iThyTraverse [getKey1] [getKey2] (iThySum GetKey1 GetKey2).
 
+ 
+  Program Definition GetKey gk1 gk2: iThy Σ :=
+    λ e1 e2, (λne Q,
+                ((⌜ e1 = do: gk1 (InjLV #()%V) ⌝%E ∗
+                ⌜ e2 = do: gk2 (InjLV #()%V) ⌝%E) ∨
+                (⌜ e1 = do: gk1 (InjRV #()%V) ⌝%E ∗
+                 ⌜ e2 = do: gk2 (InjRV #()%V) ⌝%E)) ∗
+                □ (Q NONEV NONEV ∗ ∀ key : vgG, Q (SOMEV key) (SOMEV key) )
+             )%I.
+  Next Obligation. solve_proper. Qed.
+
   (* Theories for auth channel interacting with the environment *)
   (*------------------------------------------------------------*)
   Program Definition SendBob : iThy Σ :=
@@ -208,7 +219,6 @@ Section handlee_verification.
                                 (iThySum (SendBobImpl γtokb γfracb γauthb btokN) (RecvAliceImpl γautha))))].
 
   Definition LblAdv : iLblThy Σ :=  [([getKey1],[getKey2], (iThySum GetKey1 GetKey2))].
-  About F_AUTH.
 
  (* Tactic Notation "foldkont" ident(k) open_constr(kctx) :=
     match goal with
@@ -220,42 +230,77 @@ Section handlee_verification.
 
   Tactic Notation "foldkont" := let k := fresh "kont" in foldkont k.*)
 
+  (* semantic types *)
+  (*------------------------------------------------------------*)
+
+  Definition sem_ty_group : sem_ty Σ := (λ v1 v2, ∃ g : vgG, ⌜ v1 = g ⌝ ∗ ⌜ v2 = g ⌝)%I.
+  Notation "'𝔾'" := sem_ty_group. 
+
+  Program Definition gkmono (gk1 gk2 : label) :=  {| pmono_prot_car := GetKey gk1 gk2; pmono_prot_prop := _ |}. 
+  Next Obligation.
+    intros ??. iIntros (????) "#HΦ ([(->&->)|(->&->)] & #(H1&H2))"; repeat iSplit; [by iLeft| |by iRight|]; iModIntro; iSplitL; try iIntros (?); by iApply "HΦ".
+  Qed. 
+
+  Definition gk (gk1 gk2 : label) := @SemSig Σ (gkmono gk1 gk2) (gk1,gk2).
+  
+  Program Definition θ gk1 gk2 := SemRow [([gk1],[gk2],gk gk1 gk2)] _.
+  Next Obligation.
+    intros ??.
+    iIntros (????) "#HΦ % % % ($&H)". iDestruct "H" as (?????) "(->&%&->&%&HX&#H)".
+    iExists _,_,_,_,_. 
+    repeat (iSplit; first done). iIntros (??) "!# HS". iApply "HΦ". by iApply "H". 
+  Qed. 
 
   (* Verification of DH_KE ≤ C[DH_real] *)
   (*------------------------------------------------------------*)
   
-  Lemma DH_KE_C_DH_real (f1 f2 : val) γtoka γtokb γfraca γfracb γautha γauthb L X :
+  Lemma DH_KE_C_DH_real (f1 f2 : val) γtoka γtokb γfraca γfracb γautha γauthb (L : sem_row Σ):
     let LblThy := LblAuthChannel γtoka atokN γtokb btokN γfraca γfracb γautha γauthb in
-    (*is_closed_expr ∅  f1 →
-    is_closed_expr ∅  f2 →*)
     token γtoka -∗
     token γtokb -∗
     own γautha (to_dfrac_agree (DfracOwn 1) #()%V) -∗
     own γauthb (to_dfrac_agree (DfracOwn 1) #()%V) -∗
-    BREL f1 #()%V ≤ f2 #()%V <|LblAdv ++ L|> {{ (λ v1 v2, ⌜v1 = #()%V ∧ v2 = #()%V⌝) }} -∗
-    BREL (DH_KE getKey1 channel1 f1 #()%V) ≤ (C getKey2 channel2 f2 DH_real #()%V) <|([getKey1], [getKey2], X) :: LblThy ++ L|> {{ (λ v1 v2, ⌜ v1 = v2 ⌝) }}.
+    sem_val_typed f1 f2 (∀ᵣ θₕ, ((sem_ty_sum 𝟙 𝟙) -{ θₕ }-> (Option 𝔾)) -{ sem_row_union θₕ L }-> 𝟙)%T -∗
+    BREL (DH_KE channel1 f1 #()%V) ≤ (C channel2 f2 DH_real #()%V) <|LblThy ++ (iLblSig_to_iLblThy L)|> {{ (λ v1 v2, ⌜ v1 = v2 ⌝) }}.
   Proof with (repeat foldkont) using G.
-    iIntros (LblThy) "Htoka Htokb Ha Hb Hff". repeat simpl.
+    iIntros (LblThy) "Htoka Htokb Ha Hb #Hff". repeat simpl.
     unfold DH_KE. unfold C. unfold DH_real. brel_pures.
     iApply brel_alloctape_l. iIntros (α) "!> Hα". brel_pures_l.
     iApply brel_alloctape_l. iIntros (β) "!> Hβ". brel_pures_l.
     iApply brel_alloc_l. iIntros (la) "!> Hla".
     iApply brel_alloc_l. iIntros (lb) "!> Hlb".
-    (*brel_pures_r.
-    do 3 rewrite subst_is_closed_empty; try done.
-    *)
+
     iDestruct "Hα" as (ns) "(%Hf & Hα)". apply map_eq_nil in Hf. simplify_eq.
     iApply brel_couple_TU; [done|]. iFrame. simpl. iIntros (a) "Hα".
     iDestruct "Hβ" as (ms) "(%Hf' & Hβ)". apply map_eq_nil in Hf'. simplify_eq.
     iApply brel_couple_TU; [done|]. iFrame "Hβ". simpl. iIntros (b) "Hβ".
 
     brel_pures_r. rewrite -Nat2Z.inj_mul.
-    do 3 brel_exp_r.
-    brel_pures_r.
-    (*do 3 rewrite subst_is_closed_empty; try done.*)
-    brel_pures_l.
-    (*rewrite subst_is_closed_empty; last done.*)
+    brel_pures'.
 
+    iApply brel_effect_l. iIntros (gk1) "!> Hgk1 !>".
+    iApply brel_effect_r. iIntros (gk2) "Hgk2 !>".
+    brel_pures'.
+    unfold sem_val_typed. simpl. iDestruct "Hff" as "#Hff".
+    set (θ := θ gk1 gk2).
+    iSpecialize ("Hff" $! θ).  
+    iDestruct "Hff" as "#Hff".
+    unfold sem_ty_arr, sem_ty_mbang. simpl.
+    iDestruct "Hff" as "#Hff". 
+    iAssert (sem_val_typed (λ: "party", do: gk1 "party")%V (λ: "party", do: gk2 "party")%V ((𝟙 + 𝟙)%T -{ θ }-> (Option 𝔾))%T) as "Hgg".
+    { iModIntro. rewrite /sem_ty_arr /sem_ty_mbang //=. iIntros (??) "!# #(%&%&[(->&->&->&->)|(->&->&->&->)])";
+        brel_pures';
+        iApply brel_introduction'; try constructor;
+        iExists _,_,[],[],_; do 2 (iSplit; [by iPureIntro|]; iSplit; [iPureIntro; apply NeutralEctx_nil|]);
+                          iSplit; try (iIntros (??) "!# H"; iApply "H").
+       - iSplit; first (iPureIntro; left; split; done); iModIntro; iSplitL; last iIntros (key); brel_pures'; iApply brel_value; iIntros "$ !>"; 
+             iExists _,_; [iLeft; by iPureIntro| iRight; iPureIntro; repeat (split; first done); by eexists].
+       - iSplit; first (iPureIntro; right; split; done); iModIntro; iSplitL; last iIntros (key); brel_pures'; iApply brel_value; iIntros "$ !>"; 
+             iExists _,_; [iLeft; by iPureIntro| iRight; iPureIntro; repeat (split; first done); by eexists]. }
+
+    unfold sem_val_typed. simpl. iDestruct "Hgg" as "#Hgg".
+    iSpecialize ("Hff" with "Hgg"). 
+    
     iApply fupd_brel.
     set (ga := (g ^+ a)%g).
     iMod (auth_upd (vgval (g ^+ a)%g) with "Ha") as "Ha".
@@ -289,8 +334,12 @@ Section handlee_verification.
     iSplitL "Hα Hla"; [iNext; iFrame; iLeft; iFrame|].
     iIntros "#Hinva".
 
-    iDestruct (brel_introduction_mono _ (LblAdv ++ LblThy ++ L) with "[][$Hff]") as "Hff".
-    { iApply to_iThy_le_intro'. simpl. eapply submseteq_trans; last apply submseteq_swap. by apply submseteq_cons. }
+    iApply brel_new_theory.
+    iApply (brel_add_label_l with "Hgk1").
+    iApply (brel_add_label_r with "Hgk2").
+
+    iDestruct (brel_introduction_mono _ ([([gk1],[gk2],GetKey gk1 gk2)] ++ LblThy ++ (iLblSig_to_iLblThy L)) with "[][$Hff]") as "Hf".
+    { iApply to_iThy_le_intro'. apply submseteq_skip. by apply submseteq_cons. }
     iApply (brel_exhaustion with "[$]"); [done|done|].
 
     (* getKey can be called multiple times, why we need induction *)
@@ -299,7 +348,7 @@ Section handlee_verification.
     
     iSplit; [iIntros (v1 v2) "!# (-> & ->)"; by brel_pures|].
     (* getKeyAlice or getKeyBob *)
-    iIntros (?????) "!# %Hk1 %Hk2 [(-> & -> & #(Hnone & Hsome))|(-> & -> & #(Hnone & Hsome))] #Hcont".
+    iIntros (?????) "!# %Hk1 %Hk2 ([(-> & ->)|(-> & ->)] & #(Hnone & Hsome)) #Hcont".
 
     1 : {
       brel_pures; [apply Hk1; set_solver|apply Hk2; set_solver|]...
@@ -315,7 +364,7 @@ Section handlee_verification.
         { iExists [a]. simpl. iFrame. done. }
         iFrame. iIntros "!>Hα _". brel_pures_l.
         iApply (brel_store_l _ _ _ [AppRCtx _; AppRCtx _] with "[$]").
-        iIntros "!> Hla". brel_pures_l.
+        iIntros "!> Hla". brel_pures'. 
         iApply (brel_exp_l [AppRCtx _]). brel_pures_l.
 
         iApply fupd_brel.
@@ -345,7 +394,7 @@ Section handlee_verification.
         
         iModIntro. 
         iApply brel_value. iIntros "$ !>".
-        brel_pures.
+        brel_pures'.
 
         iApply (brel_bind' [_] [_]); [iApply traversable_to_iThy|].
         iApply (brel_introduction' [channel1] [channel2]).
@@ -524,312 +573,312 @@ Section handlee_verification.
     
   
 
-  Lemma C_DH_real_DH_KE (f1 f2 : val) γtoka γtokb γfraca γfracb γautha γauthb L X  :
-    let LblThy := LblAuthChannel γtoka atokN γtokb btokN γfraca γfracb γautha γauthb in
-        (* is_closed_expr ∅ f1 →
-         is_closed_expr ∅ f2 →*)
-         token γtoka -∗
-         token γtokb -∗
-           own γautha (to_dfrac_agree (DfracOwn 1) #()%V) -∗
-           own γauthb (to_dfrac_agree (DfracOwn 1) #()%V) -∗
-           BREL f1 #()%V ≤ f2 #()%V <|LblAdv ++ L|> {{ (λ v1 v2, ⌜v1 = #()%V ∧ v2 = #()%V⌝) }} -∗
-           BREL (C getKey1 channel1 f1 DH_real #()%V) ≤ (DH_KE getKey2 channel2 f2 #()%V)  <|([getKey1],[getKey2], X) :: LblThy ++ L|> {{ (λ v1 v2, ⌜ v1 = v2 ⌝) }}.
-  Proof using G.
-    iIntros (LblThy) "Htoka Htokb Ha Hb Hff".
-    unfold C. unfold DH_KE.
-    iApply brel_alloctape_r. iIntros (α) "Hα". brel_pures_r.
-    (*rewrite subst_is_closed_empty; try done.*)
-    iApply brel_alloctape_r. iIntros (β) "Hβ". brel_pures_r.
-    (*rewrite subst_is_closed_empty; try done.*)
-    iApply brel_alloc_r. iIntros (la) "Hla". brel_pures_r.
-    (*rewrite subst_is_closed_empty; try done.*)
-    iApply brel_alloc_r. iIntros (lb) "Hlb". brel_pures_r. 
-    (*rewrite subst_is_closed_empty; try done.*)
-    iApply brel_couple_UT. 1: auto. iFrame "Hα". simpl. iSplit => //. iIntros (a ?) "!> Hα".
-    iApply brel_couple_UT. 1: auto. iFrame "Hβ". simpl. iSplit => //. iIntros (b ?) "!> Hβ".
-    
-    brel_pures_l. rewrite -Nat2Z.inj_mul.
-    do 3 brel_exp_l.
-    brel_pures_l.
-    (*do 3 rewrite subst_is_closed_empty; try done.*)
-        
-    iApply fupd_brel.
-    set (ga := (g ^+ a)%g).
-    iMod (auth_upd (vgval (g ^+ a)%g) with "Ha") as "Ha".
-    iMod (auth_upd (vgval $ g ^+ b)%g with "Hb") as "Hb".
-    iMod (auth_persist with "Ha") as "#Ha".
-    iMod (auth_persist with "Hb") as "#Hb".
-    iModIntro.
-  
-    iApply fupd_brel.
-    iMod (inv_alloc atokN _ (token γtoka ∨ own γfraca DfracDiscarded)%I with "[Htoka]") as "#Hinvta".
-    { iNext; iLeft;iFrame. }
-    iMod (inv_alloc btokN _ (token γtokb ∨ own γfracb DfracDiscarded)%I with "[Htokb]") as "#Hinvtb".
-    { iNext; iFrame. }
-    iModIntro.    
-    iApply (brel_na_alloc
-              ((β ↪ₛN (n; [b]) ∗ lb ↦ₛ NONEV)
-               ∨ (β ↪ₛ□ (n; [])
-                  ∗ lb ↦ₛ□ SOMEV #b)
-              )%I
-              betaN).
-    iSplitL "Hβ Hlb"; [iNext; iFrame; iLeft; iFrame|].
-    iIntros "#Hinvb".
-    
-    iApply (brel_na_alloc
-              ((α ↪ₛN (n; [a]) ∗ la ↦ₛ NONEV)
-               ∨ (α ↪ₛ□ (n; [])
-                  ∗ la ↦ₛ□ SOMEV #a))%I
-              alphaN).
-    iSplitL "Hα Hla"; [iNext; iFrame; iLeft; iFrame|].
-    iIntros "#Hinva".
-    
-    iDestruct (brel_introduction_mono _ (LblAdv ++ LblThy ++ L) with "[][$Hff]") as "Hff".
-    { iApply to_iThy_le_intro'. simpl. eapply submseteq_trans; last apply submseteq_swap. by apply submseteq_cons. }
-    iApply (brel_exhaustion with "[$]"); [done|done|].
-
-    iLöb as "IH".
-    
-    
-    iSplit; [iIntros (v1 v2) "!# (-> & ->)"; by brel_pures|].
-    
-    iIntros (?????) "!# %Hk1 %Hk2 [(-> & -> & #(Hnone & Hsome))|(-> & -> & #(Hnone & Hsome))] #Hcont".
-    
-     1 : {
-       brel_pures; [apply Hk1; set_solver|apply Hk2; set_solver|].
-       iApply (brel_na_inv _ _ alphaN ); [set_solver|].
-       iFrame "Hinva". 
-       iIntros "([(>Hα & >Hla) | (#>Hα & #>Hla)] & Hclose)".
-       - iApply (brel_load_r _ _ _ _ [AppRCtx _; CaseCtx _ _] with "Hla").
-         iIntros "Hla". brel_pures_r.
-         (* iAssert (α ↪ₛN (n; [a]))%I with "[Hα]" as "Hα".
-            { iExists [a]. simpl. iFrame. done. } *)
-         iApply (brel_rand_r _ [AppRCtx _; AppRCtx _] with "Hα").
-         iIntros "Hα _". brel_pures_r.
-         iApply (brel_store_r _ _ _ _[AppRCtx _; AppRCtx _] with "Hla").
-         iIntros "Hla".
-         brel_pures_r. 
-         iApply (brel_exp_r [AppRCtx _]). brel_pures_r.
-     
-         iApply fupd_brel.
-         iMod (ghost_map_elem_persist with "Hla") as "#Hla".
-         iDestruct "Hα" as (ns) "(%Hf & Hα)". apply map_eq_nil in Hf. simplify_eq.
-         iMod (ghost_map_elem_persist with "Hα") as "#Hα".
-         iModIntro.
-         iApply brel_na_close. iFrame.
-         iSplitL; [iNext; iRight; iFrame "#"|].
-         
-         (* Send (gA, bob) *)
-         iApply (brel_bind' [_] [_]); [iApply traversable_to_iThy|].
-         iApply (brel_introduction' [channel1] [channel2]).
-         { apply elem_of_cons. right. apply list_elem_of_here. }
-         
-         iExists _, _, [], [], _. do 2 (iSplit; [done|]; iSplit; [iPureIntro; apply _|]).
-         iSplitL; [|by iIntros "!>" (??) "H"; iApply "H"].
-         iLeft. iLeft. 
-         iExists _, _.
-         iSplitL.
-         { iMod (inv_acc with "Hinvta") as "([>Htok | >#Hfrac'] & Hclose)"; try done.
-           - iModIntro. iLeft.
-             iIntros. iFrame. iMod ("Hclose" with "[$]") as "_". iFrame "#". 
-             by iModIntro.
-           - iModIntro. iRight. by iMod ("Hclose" with "[$]") as "_". }
-         iSplit; first ( do 2 (iSplit; try (iPureIntro; done))).
-         iModIntro.
-         iApply brel_value. iIntros "$ !>".
-         brel_pures.
-         
-         (* Recv bob (either none or some) *)
-         iApply (brel_bind' [_] [_]); [iApply traversable_to_iThy|].
-         iApply (brel_introduction' [channel1] [channel2]).
-         { apply elem_of_cons. right. apply list_elem_of_here. }
-         iExists _, _, [], [], _. do 2 (iSplit; [done|]; iSplit; [iPureIntro; apply _|]).
-         iSplitL; [|by iIntros "!>" (??) "H"; iApply "H"].
-         iLeft. iRight.
-         do 2 (iSplit; try (iPureIntro; done)).
-         iModIntro.
-         iSplitL.
-                 
-         (* Recv bob = None *)
-         + iApply brel_value. iIntros "$ !>".
-           brel_pures.
-           iDestruct ("Hcont" with "Hnone") as "Hkk".
-           iApply (brel_exhaustion _ _ [_] [_] with "[$]"); [done|done|].
-           iApply "IH".
+  (* Lemma C_DH_real_DH_KE (f1 f2 : val) γtoka γtokb γfraca γfracb γautha γauthb L X  :
+       let LblThy := LblAuthChannel γtoka atokN γtokb btokN γfraca γfracb γautha γauthb in
+           (* is_closed_expr ∅ f1 →
+            is_closed_expr ∅ f2 →*)
+            token γtoka -∗
+            token γtokb -∗
+              own γautha (to_dfrac_agree (DfracOwn 1) #()%V) -∗
+              own γauthb (to_dfrac_agree (DfracOwn 1) #()%V) -∗
+              BREL f1 #()%V ≤ f2 #()%V <|LblAdv ++ L|> {{ (λ v1 v2, ⌜v1 = #()%V ∧ v2 = #()%V⌝) }} -∗
+              BREL (C getKey1 channel1 f1 DH_real #()%V) ≤ (DH_KE getKey2 channel2 f2 #()%V)  <|([getKey1],[getKey2], X) :: LblThy ++ L|> {{ (λ v1 v2, ⌜ v1 = v2 ⌝) }}.
+     Proof using G.
+       iIntros (LblThy) "Htoka Htokb Ha Hb Hff".
+       unfold C. unfold DH_KE.
+       iApply brel_alloctape_r. iIntros (α) "Hα". brel_pures_r.
+       (*rewrite subst_is_closed_empty; try done.*)
+       iApply brel_alloctape_r. iIntros (β) "Hβ". brel_pures_r.
+       (*rewrite subst_is_closed_empty; try done.*)
+       iApply brel_alloc_r. iIntros (la) "Hla". brel_pures_r.
+       (*rewrite subst_is_closed_empty; try done.*)
+       iApply brel_alloc_r. iIntros (lb) "Hlb". brel_pures_r. 
+       (*rewrite subst_is_closed_empty; try done.*)
+       iApply brel_couple_UT. 1: auto. iFrame "Hα". simpl. iSplit => //. iIntros (a ?) "!> Hα".
+       iApply brel_couple_UT. 1: auto. iFrame "Hβ". simpl. iSplit => //. iIntros (b ?) "!> Hβ".
+       
+       brel_pures_l. rewrite -Nat2Z.inj_mul.
+       do 3 brel_exp_l.
+       brel_pures_l.
+       (*do 3 rewrite subst_is_closed_empty; try done.*)
            
-         (* Recv bob = Some gB *)
-         + iIntros (m) "Ha'".
-           iDestruct (auth_agree with "[$Hb] [$Ha']") as "<-".
-           iApply brel_value. iIntros "$ !>".
-           brel_pures. brel_exp_r.
-           rewrite -expgM. rewrite -ssrnat.multE.
-           rewrite -Nat.mul_comm.
-           iDestruct ("Hcont" with "Hsome") as "Hkk".
-           iApply (brel_exhaustion _ _ [_] [_] with "[$]"); [done|done|].
-           iApply "IH".
-
-       - iApply brel_na_close. iFrame. iSplitL; [iRight; iFrame "#"|].
-         iApply (brel_load_r with "Hla"). iIntros "_". brel_pures.
-         brel_exp_r. brel_pures.
-         
-         (* Send (gA, bob) *)
-         iApply (brel_bind' [_] [_]); [iApply traversable_to_iThy|].
-         iApply (brel_introduction' [channel1] [channel2]).
-         { apply elem_of_cons. right. apply list_elem_of_here. }
-         iExists _, _, [], [], _. do 2 (iSplit; [done|]; iSplit; [iPureIntro; apply _|]).
-         iSplitL; [|by iIntros "!>" (??) "H"; iApply "H"].
-         iLeft. iLeft.
-         iExists _, _.
-         iSplitL.
-         { iMod (inv_acc with "Hinvta") as "([>Htok | >#Hfrac'] & Hclose)"; try done.
-           - iModIntro. iLeft.
-             iIntros. iFrame. iMod ("Hclose" with "[$]") as "_". iFrame "#". 
-             by iModIntro. 
-           - iModIntro. iRight. iFrame "#".
-             iApply "Hclose". iNext.
-             by iRight. }
-         iSplit; first (iSplit; try (iPureIntro; done)).
-         iModIntro.
-         iApply brel_value. iIntros "$ !>".
-         brel_pures.
-         
-         iApply (brel_bind' [_] [_]); [iApply traversable_to_iThy|].
-         iApply (brel_introduction' [channel1] [channel2]).
-         { apply elem_of_cons. right. apply list_elem_of_here. }
-         iExists _, _, [], [], _. do 2 (iSplit; [done|]; iSplit; [iPureIntro; apply _|]).
-         iSplitL; [|by iIntros "!>" (??) "H"; iApply "H"].
-         iLeft. iRight.
-         do 2 (iSplit; try (iPureIntro; done)).
-         iModIntro.
-         iSplitL.
-
-         (* Recv bob = None *)
-         + iApply brel_value. iIntros "$ !>".
-           brel_pures.
-           iDestruct ("Hcont" with "Hnone") as "Hkk".
-           iApply (brel_exhaustion _ _ [_] [_] with "[$]"); [done|done|].
-           iApply "IH".
-
-         (* Recv bob = Some gB *)
-         + iIntros (m) "Ha'".
-           iDestruct (auth_agree with "[$Hb] [$Ha']") as "<-".
-           iApply brel_value. iIntros "$ !>".
-           brel_pures. brel_exp_r. brel_pures.
-           rewrite -expgM. rewrite -ssrnat.multE.
-           rewrite -Nat.mul_comm.
-           iDestruct ("Hcont" with "Hsome") as "Hkk".
-           iApply (brel_exhaustion _ _ [_] [_] with "[$]"); [done|done|].
-           iApply "IH". }
-  
-     1 : {
-       brel_pures; [apply Hk1; set_solver|apply Hk2; set_solver|].
-       iApply (brel_bind' [_] [_]); [iApply traversable_to_iThy|].
-       iApply brel_introduction'.
-       { apply elem_of_cons. right. apply list_elem_of_here. }
-       iExists _, _, [], [], _. do 2 (iSplit; [done|]; iSplit; [iPureIntro; apply _|]).
-       iSplitL; [|by iIntros "!>" (??) "H"; iApply "H"].
-       iRight. iRight.
-       do 2 (iSplit; try (iPureIntro; done)).
+       iApply fupd_brel.
+       set (ga := (g ^+ a)%g).
+       iMod (auth_upd (vgval (g ^+ a)%g) with "Ha") as "Ha".
+       iMod (auth_upd (vgval $ g ^+ b)%g with "Hb") as "Hb".
+       iMod (auth_persist with "Ha") as "#Ha".
+       iMod (auth_persist with "Hb") as "#Hb".
        iModIntro.
-       iSplitL.
-       { iApply brel_value. iIntros "$ !>".
-         brel_pures.
-         iDestruct ("Hcont" with "Hnone") as "Hkk".
-         iApply (brel_exhaustion _ _ [_] [_] with "[$]"); [done|done|].
-         iApply "IH". }
-       iIntros (m) "Hb'".
-       iDestruct (auth_agree with "[$Ha] [$Hb']") as "<-".
-       iApply brel_value. iIntros "$ !>".
-       brel_pures.
-
-       iApply (brel_na_inv _ _ betaN ); [set_solver|].
-       iFrame "Hinvb". 
-       iIntros "(>[(Hβ & Hlb) | #(Hβ & Hlb)] & Hclose)".
-       - iApply (brel_load_r _ _ _ _ [AppRCtx _; CaseCtx _ _] with "[$]").
-         iIntros "Hlb". brel_pures_r.
-         (* iAssert (β ↪ₛN (n; [fin_to_nat b]))%I with "[Hβ]" as "Hβ".
-            { iExists _. simpl. iFrame. done. } *)
-         iApply (brel_rand_r _ [AppRCtx _; AppRCtx _] with "[$]").
-         iIntros "Hβ _". brel_pures_r.
-         iApply (brel_store_r _ _ _ _[AppRCtx _; AppRCtx _] with "Hlb").
-         iIntros "Hlb".
-         brel_pures_r. 
-         iApply (brel_exp_r [AppRCtx _]). brel_pures_r.
-         iApply fupd_brel.
-         iMod (ghost_map_elem_persist with "Hlb") as "#Hlb".
-         iDestruct "Hβ" as (ns) "(%Hf & Hβ)". apply map_eq_nil in Hf. simplify_eq.
-         iMod (ghost_map_elem_persist with "Hβ") as "#Hβ".
-         iModIntro.
-         iApply brel_na_close. iFrame.
-         iSplitL; [iNext; iRight; iFrame "#"|].
-
-         (* Send (gB, alice) *)
-         iApply (brel_bind' [_] [_]); [by iApply traversable_to_iThy|].
-         iApply brel_introduction'. { apply elem_of_cons. right. apply list_elem_of_here. }
-         iExists _, _, [], [], _. do 2 (iSplit; [done|]; iSplit; [iPureIntro; apply _|]).
-         iSplitL; [|by iIntros "!>" (??) "H"; iApply "H"].
-         iRight. iLeft. 
-         iExists _,_.
-         iSplitL.
-         { iMod (inv_acc with "Hinvtb") as "([>Htok | >#Hfrac'] & Hclose)"; try done.
-           - iModIntro. iLeft.
-             iIntros. iFrame. iMod ("Hclose" with "[$]") as "_". iFrame "#". 
-             by iModIntro. 
-           - iModIntro. iRight. by iMod ("Hclose" with "[$]") as "_". }
-         iSplit; first ( do 2 (iSplit; try (iPureIntro; done))).
-         iModIntro.
-         iApply brel_value. iIntros "$ !>".
-         brel_pures.
-         rewrite -expgM. rewrite -ssrnat.multE.
-         rewrite -Nat.mul_comm.
-
-         iDestruct ("Hcont" with "Hsome") as "Hkk".
-         iApply (brel_exhaustion _ _ [_] [_] with "[$]"); [done|done|].
-         iApply "IH".
-         
-       - iApply brel_na_close. iFrame. iSplitL; [iRight; iFrame "#"|].
-         iApply (brel_load_r with "Hlb"). iIntros "_". brel_pures.
-         brel_exp_r. brel_pures.
-         
-         (* Send (gB, alice) *)
-         iApply (brel_bind' [AppRCtx _] [AppRCtx _]); [by iApply traversable_to_iThy|].
-         iApply brel_introduction'. { apply elem_of_cons. right. apply list_elem_of_here. }
-         iExists _, _, [], [], _. do 2 (iSplit; [done|]; iSplit; [iPureIntro; apply _|]).
-         iSplitL; [|by iIntros "!>" (??) "H"; iApply "H"].
-         iRight. iLeft.
-         iExists _,_.
-         iSplitL.
-         { iMod (inv_acc with "Hinvtb") as "([>Htok | >#Hfrac'] & Hclose)"; try done.
-           - iModIntro. iLeft.
-             iIntros. iFrame. iMod ("Hclose" with "[$]") as "_". iFrame "#". 
-             by iModIntro. 
-           - iModIntro. iRight. by iMod ("Hclose" with "[$]") as "_". }
-         iSplit; first ( do 2 (iSplit; try (iPureIntro; done))).
-         
-         iModIntro. 
-         iApply brel_value. iIntros "$ !>".
-         brel_pures.
-         rewrite -expgM. rewrite -ssrnat.multE.
-         rewrite -Nat.mul_comm.
-
-         iDestruct ("Hcont" with "Hsome") as "Hkk".
-         iApply (brel_exhaustion _ _ [_] [_] with "[$]"); [done|done|].
-         iApply "IH". }
-  Qed.      
+     
+       iApply fupd_brel.
+       iMod (inv_alloc atokN _ (token γtoka ∨ own γfraca DfracDiscarded)%I with "[Htoka]") as "#Hinvta".
+       { iNext; iLeft;iFrame. }
+       iMod (inv_alloc btokN _ (token γtokb ∨ own γfracb DfracDiscarded)%I with "[Htokb]") as "#Hinvtb".
+       { iNext; iFrame. }
+       iModIntro.    
+       iApply (brel_na_alloc
+                 ((β ↪ₛN (n; [b]) ∗ lb ↦ₛ NONEV)
+                  ∨ (β ↪ₛ□ (n; [])
+                     ∗ lb ↦ₛ□ SOMEV #b)
+                 )%I
+                 betaN).
+       iSplitL "Hβ Hlb"; [iNext; iFrame; iLeft; iFrame|].
+       iIntros "#Hinvb".
+       
+       iApply (brel_na_alloc
+                 ((α ↪ₛN (n; [a]) ∗ la ↦ₛ NONEV)
+                  ∨ (α ↪ₛ□ (n; [])
+                     ∗ la ↦ₛ□ SOMEV #a))%I
+                 alphaN).
+       iSplitL "Hα Hla"; [iNext; iFrame; iLeft; iFrame|].
+       iIntros "#Hinva".
+       
+       iDestruct (brel_introduction_mono _ (LblAdv ++ LblThy ++ L) with "[][$Hff]") as "Hff".
+       { iApply to_iThy_le_intro'. simpl. eapply submseteq_trans; last apply submseteq_swap. by apply submseteq_cons. }
+       iApply (brel_exhaustion with "[$]"); [done|done|].
+     
+       iLöb as "IH".
+       
+       
+       iSplit; [iIntros (v1 v2) "!# (-> & ->)"; by brel_pures|].
+       
+       iIntros (?????) "!# %Hk1 %Hk2 [(-> & -> & #(Hnone & Hsome))|(-> & -> & #(Hnone & Hsome))] #Hcont".
+       
+        1 : {
+          brel_pures; [apply Hk1; set_solver|apply Hk2; set_solver|].
+          iApply (brel_na_inv _ _ alphaN ); [set_solver|].
+          iFrame "Hinva". 
+          iIntros "([(>Hα & >Hla) | (#>Hα & #>Hla)] & Hclose)".
+          - iApply (brel_load_r _ _ _ _ [AppRCtx _; CaseCtx _ _] with "Hla").
+            iIntros "Hla". brel_pures_r.
+            (* iAssert (α ↪ₛN (n; [a]))%I with "[Hα]" as "Hα".
+               { iExists [a]. simpl. iFrame. done. } *)
+            iApply (brel_rand_r _ [AppRCtx _; AppRCtx _] with "Hα").
+            iIntros "Hα _". brel_pures_r.
+            iApply (brel_store_r _ _ _ _[AppRCtx _; AppRCtx _] with "Hla").
+            iIntros "Hla".
+            brel_pures_r. 
+            iApply (brel_exp_r [AppRCtx _]). brel_pures_r.
+        
+            iApply fupd_brel.
+            iMod (ghost_map_elem_persist with "Hla") as "#Hla".
+            iDestruct "Hα" as (ns) "(%Hf & Hα)". apply map_eq_nil in Hf. simplify_eq.
+            iMod (ghost_map_elem_persist with "Hα") as "#Hα".
+            iModIntro.
+            iApply brel_na_close. iFrame.
+            iSplitL; [iNext; iRight; iFrame "#"|].
+            
+            (* Send (gA, bob) *)
+            iApply (brel_bind' [_] [_]); [iApply traversable_to_iThy|].
+            iApply (brel_introduction' [channel1] [channel2]).
+            { apply elem_of_cons. right. apply list_elem_of_here. }
+            
+            iExists _, _, [], [], _. do 2 (iSplit; [done|]; iSplit; [iPureIntro; apply _|]).
+            iSplitL; [|by iIntros "!>" (??) "H"; iApply "H"].
+            iLeft. iLeft. 
+            iExists _, _.
+            iSplitL.
+            { iMod (inv_acc with "Hinvta") as "([>Htok | >#Hfrac'] & Hclose)"; try done.
+              - iModIntro. iLeft.
+                iIntros. iFrame. iMod ("Hclose" with "[$]") as "_". iFrame "#". 
+                by iModIntro.
+              - iModIntro. iRight. by iMod ("Hclose" with "[$]") as "_". }
+            iSplit; first ( do 2 (iSplit; try (iPureIntro; done))).
+            iModIntro.
+            iApply brel_value. iIntros "$ !>".
+            brel_pures.
+            
+            (* Recv bob (either none or some) *)
+            iApply (brel_bind' [_] [_]); [iApply traversable_to_iThy|].
+            iApply (brel_introduction' [channel1] [channel2]).
+            { apply elem_of_cons. right. apply list_elem_of_here. }
+            iExists _, _, [], [], _. do 2 (iSplit; [done|]; iSplit; [iPureIntro; apply _|]).
+            iSplitL; [|by iIntros "!>" (??) "H"; iApply "H"].
+            iLeft. iRight.
+            do 2 (iSplit; try (iPureIntro; done)).
+            iModIntro.
+            iSplitL.
+                    
+            (* Recv bob = None *)
+            + iApply brel_value. iIntros "$ !>".
+              brel_pures.
+              iDestruct ("Hcont" with "Hnone") as "Hkk".
+              iApply (brel_exhaustion _ _ [_] [_] with "[$]"); [done|done|].
+              iApply "IH".
+              
+            (* Recv bob = Some gB *)
+            + iIntros (m) "Ha'".
+              iDestruct (auth_agree with "[$Hb] [$Ha']") as "<-".
+              iApply brel_value. iIntros "$ !>".
+              brel_pures. brel_exp_r.
+              rewrite -expgM. rewrite -ssrnat.multE.
+              rewrite -Nat.mul_comm.
+              iDestruct ("Hcont" with "Hsome") as "Hkk".
+              iApply (brel_exhaustion _ _ [_] [_] with "[$]"); [done|done|].
+              iApply "IH".
+     
+          - iApply brel_na_close. iFrame. iSplitL; [iRight; iFrame "#"|].
+            iApply (brel_load_r with "Hla"). iIntros "_". brel_pures.
+            brel_exp_r. brel_pures.
+            
+            (* Send (gA, bob) *)
+            iApply (brel_bind' [_] [_]); [iApply traversable_to_iThy|].
+            iApply (brel_introduction' [channel1] [channel2]).
+            { apply elem_of_cons. right. apply list_elem_of_here. }
+            iExists _, _, [], [], _. do 2 (iSplit; [done|]; iSplit; [iPureIntro; apply _|]).
+            iSplitL; [|by iIntros "!>" (??) "H"; iApply "H"].
+            iLeft. iLeft.
+            iExists _, _.
+            iSplitL.
+            { iMod (inv_acc with "Hinvta") as "([>Htok | >#Hfrac'] & Hclose)"; try done.
+              - iModIntro. iLeft.
+                iIntros. iFrame. iMod ("Hclose" with "[$]") as "_". iFrame "#". 
+                by iModIntro. 
+              - iModIntro. iRight. iFrame "#".
+                iApply "Hclose". iNext.
+                by iRight. }
+            iSplit; first (iSplit; try (iPureIntro; done)).
+            iModIntro.
+            iApply brel_value. iIntros "$ !>".
+            brel_pures.
+            
+            iApply (brel_bind' [_] [_]); [iApply traversable_to_iThy|].
+            iApply (brel_introduction' [channel1] [channel2]).
+            { apply elem_of_cons. right. apply list_elem_of_here. }
+            iExists _, _, [], [], _. do 2 (iSplit; [done|]; iSplit; [iPureIntro; apply _|]).
+            iSplitL; [|by iIntros "!>" (??) "H"; iApply "H"].
+            iLeft. iRight.
+            do 2 (iSplit; try (iPureIntro; done)).
+            iModIntro.
+            iSplitL.
+     
+            (* Recv bob = None *)
+            + iApply brel_value. iIntros "$ !>".
+              brel_pures.
+              iDestruct ("Hcont" with "Hnone") as "Hkk".
+              iApply (brel_exhaustion _ _ [_] [_] with "[$]"); [done|done|].
+              iApply "IH".
+     
+            (* Recv bob = Some gB *)
+            + iIntros (m) "Ha'".
+              iDestruct (auth_agree with "[$Hb] [$Ha']") as "<-".
+              iApply brel_value. iIntros "$ !>".
+              brel_pures. brel_exp_r. brel_pures.
+              rewrite -expgM. rewrite -ssrnat.multE.
+              rewrite -Nat.mul_comm.
+              iDestruct ("Hcont" with "Hsome") as "Hkk".
+              iApply (brel_exhaustion _ _ [_] [_] with "[$]"); [done|done|].
+              iApply "IH". }
+     
+        1 : {
+          brel_pures; [apply Hk1; set_solver|apply Hk2; set_solver|].
+          iApply (brel_bind' [_] [_]); [iApply traversable_to_iThy|].
+          iApply brel_introduction'.
+          { apply elem_of_cons. right. apply list_elem_of_here. }
+          iExists _, _, [], [], _. do 2 (iSplit; [done|]; iSplit; [iPureIntro; apply _|]).
+          iSplitL; [|by iIntros "!>" (??) "H"; iApply "H"].
+          iRight. iRight.
+          do 2 (iSplit; try (iPureIntro; done)).
+          iModIntro.
+          iSplitL.
+          { iApply brel_value. iIntros "$ !>".
+            brel_pures.
+            iDestruct ("Hcont" with "Hnone") as "Hkk".
+            iApply (brel_exhaustion _ _ [_] [_] with "[$]"); [done|done|].
+            iApply "IH". }
+          iIntros (m) "Hb'".
+          iDestruct (auth_agree with "[$Ha] [$Hb']") as "<-".
+          iApply brel_value. iIntros "$ !>".
+          brel_pures.
+     
+          iApply (brel_na_inv _ _ betaN ); [set_solver|].
+          iFrame "Hinvb". 
+          iIntros "(>[(Hβ & Hlb) | #(Hβ & Hlb)] & Hclose)".
+          - iApply (brel_load_r _ _ _ _ [AppRCtx _; CaseCtx _ _] with "[$]").
+            iIntros "Hlb". brel_pures_r.
+            (* iAssert (β ↪ₛN (n; [fin_to_nat b]))%I with "[Hβ]" as "Hβ".
+               { iExists _. simpl. iFrame. done. } *)
+            iApply (brel_rand_r _ [AppRCtx _; AppRCtx _] with "[$]").
+            iIntros "Hβ _". brel_pures_r.
+            iApply (brel_store_r _ _ _ _[AppRCtx _; AppRCtx _] with "Hlb").
+            iIntros "Hlb".
+            brel_pures_r. 
+            iApply (brel_exp_r [AppRCtx _]). brel_pures_r.
+            iApply fupd_brel.
+            iMod (ghost_map_elem_persist with "Hlb") as "#Hlb".
+            iDestruct "Hβ" as (ns) "(%Hf & Hβ)". apply map_eq_nil in Hf. simplify_eq.
+            iMod (ghost_map_elem_persist with "Hβ") as "#Hβ".
+            iModIntro.
+            iApply brel_na_close. iFrame.
+            iSplitL; [iNext; iRight; iFrame "#"|].
+     
+            (* Send (gB, alice) *)
+            iApply (brel_bind' [_] [_]); [by iApply traversable_to_iThy|].
+            iApply brel_introduction'. { apply elem_of_cons. right. apply list_elem_of_here. }
+            iExists _, _, [], [], _. do 2 (iSplit; [done|]; iSplit; [iPureIntro; apply _|]).
+            iSplitL; [|by iIntros "!>" (??) "H"; iApply "H"].
+            iRight. iLeft. 
+            iExists _,_.
+            iSplitL.
+            { iMod (inv_acc with "Hinvtb") as "([>Htok | >#Hfrac'] & Hclose)"; try done.
+              - iModIntro. iLeft.
+                iIntros. iFrame. iMod ("Hclose" with "[$]") as "_". iFrame "#". 
+                by iModIntro. 
+              - iModIntro. iRight. by iMod ("Hclose" with "[$]") as "_". }
+            iSplit; first ( do 2 (iSplit; try (iPureIntro; done))).
+            iModIntro.
+            iApply brel_value. iIntros "$ !>".
+            brel_pures.
+            rewrite -expgM. rewrite -ssrnat.multE.
+            rewrite -Nat.mul_comm.
+     
+            iDestruct ("Hcont" with "Hsome") as "Hkk".
+            iApply (brel_exhaustion _ _ [_] [_] with "[$]"); [done|done|].
+            iApply "IH".
+            
+          - iApply brel_na_close. iFrame. iSplitL; [iRight; iFrame "#"|].
+            iApply (brel_load_r with "Hlb"). iIntros "_". brel_pures.
+            brel_exp_r. brel_pures.
+            
+            (* Send (gB, alice) *)
+            iApply (brel_bind' [AppRCtx _] [AppRCtx _]); [by iApply traversable_to_iThy|].
+            iApply brel_introduction'. { apply elem_of_cons. right. apply list_elem_of_here. }
+            iExists _, _, [], [], _. do 2 (iSplit; [done|]; iSplit; [iPureIntro; apply _|]).
+            iSplitL; [|by iIntros "!>" (??) "H"; iApply "H"].
+            iRight. iLeft.
+            iExists _,_.
+            iSplitL.
+            { iMod (inv_acc with "Hinvtb") as "([>Htok | >#Hfrac'] & Hclose)"; try done.
+              - iModIntro. iLeft.
+                iIntros. iFrame. iMod ("Hclose" with "[$]") as "_". iFrame "#". 
+                by iModIntro. 
+              - iModIntro. iRight. by iMod ("Hclose" with "[$]") as "_". }
+            iSplit; first ( do 2 (iSplit; try (iPureIntro; done))).
+            
+            iModIntro. 
+            iApply brel_value. iIntros "$ !>".
+            brel_pures.
+            rewrite -expgM. rewrite -ssrnat.multE.
+            rewrite -Nat.mul_comm.
+     
+            iDestruct ("Hcont" with "Hsome") as "Hkk".
+            iApply (brel_exhaustion _ _ [_] [_] with "[$]"); [done|done|].
+            iApply "IH". }
+     Qed.       *)
      
      
      
      (* Verification of F_AUTH ≤ F_AUTH *)
      (*------------------------------------------------------------*)
      
-  Lemma F_AUTH_F_AUTH (f1 f2 : val) γtoka γtokb γfraca γfracb γautha γauthb X L :
+  Lemma F_AUTH_F_AUTH (f1 f2 : val) γtoka γtokb γfraca γfracb γautha γauthb L :
     let LblThy := LblAuthChannel γtoka atokN γtokb btokN γfraca γfracb γautha γauthb in
     (*is_closed_expr ∅ f1 →
     is_closed_expr ∅ f2 →*)
     own γfraca (DfracOwn 1) -∗
     own γfracb (DfracOwn 1) -∗
-    BREL f1 #()%V ≤ f2 #()%V <|([getKey1],[getKey2], X) :: LblThy ++ L|> {{ (λ v1 v2, ⌜ v1 = v2 ⌝) }} -∗
-    BREL F_AUTH channel1 leakauth1 f1 #()%V ≤ F_AUTH channel2 leakauth2 f2 #()%V <|LblEnv ++ ([getKey1],[getKey2], X) :: L |> {{ (λ v1 v2, ⌜ v1 = v2 ⌝) }}.
+    BREL f1 #()%V ≤ f2 #()%V <| LblThy ++ L|> {{ (λ v1 v2, ⌜ v1 = v2 ⌝) }} -∗
+    BREL F_AUTH channel1 leakauth1 f1 #()%V ≤ F_AUTH channel2 leakauth2 f2 #()%V <|LblEnv ++  L |> {{ (λ v1 v2, ⌜ v1 = v2 ⌝) }}.
   Proof using G. 
   (*   iIntros (LblThy Hf1closed Hf2closed) "Hfraca Hfracb Hff".
        iApply brel_alloc_l. iIntros (l1) "!> Hl1".
@@ -1037,11 +1086,10 @@ Section handlee_verification.
 
   (* Verification of F_AUTH[DH_KE] ≤ F_AUTH[C[DH_real]] *)
   (*------------------------------------------------------------*)
-  Lemma F_AUTH_DH_KE_FAUTH_C_DH_real (f1 f2 : val) L X :
-    (*is_closed_expr ∅ f1 →
-    is_closed_expr ∅ f2 →*)
-    BREL f1 #()%V ≤ f2 #()%V <|LblAdv ++ L|> {{ λ v1 v2, ⌜ v1 = #()%V ∧ v2 = #()%V ⌝ }} -∗
-    BREL F_AUTH channel1 leakauth1 (DH_KE getKey1 channel1 f1) #()%V ≤ F_AUTH channel2 leakauth2 (C getKey2 channel2 f2 DH_real) #()%V <|LblEnv ++ ([getKey1],[getKey2], X) :: L|> {{ λ v1 v2, ⌜ v1 = v2 ⌝ }}.
+  (* TODO: adjust the proof for the new form of DHKE *)
+  Lemma F_AUTH_DH_KE_FAUTH_C_DH_real (f1 f2 : val) L :
+    sem_val_typed f1 f2 (∀ᵣ θₕ, ((sem_ty_sum 𝟙 𝟙) -{ θₕ }-> (Option 𝔾)) -{ sem_row_union θₕ L }-> 𝟙)%T -∗
+    BREL F_AUTH channel1 leakauth1 (DH_KE channel1 f1) #()%V ≤ F_AUTH channel2 leakauth2 (C channel2 f2 DH_real) #()%V <|LblEnv ++ (iLblSig_to_iLblThy L)|> {{ λ v1 v2, ⌜ v1 = v2 ⌝ }}.
   Proof using G inG0 inG1 inG2.
     iIntros "Hff".
     
@@ -1055,24 +1103,20 @@ Section handlee_verification.
     iModIntro.
 
     (*iApply F_AUTH_F_AUTH.*)
-    About DH_KE.
-    Print F_AUTH_F_AUTH.
-    
+  (*   iApply (F_AUTH_F_AUTH (DH_KE channel1 f1) (C channel2 f2)).
+       iApply (F_AUTH_F_AUTH with "[$][$]"); [| |].
+       1,2 : simpl; repeat (rewrite andb_True; split); try set_solver; eauto using vunit_closed, vmult_closed, g_closed;
+             by apply is_closed_weaken_empty. 
+       by iApply (DH_KE_C_DH_real with "[$][$][$][$]"); eauto.
+     Qed. *)
+  Admitted. 
 
-    iApply (F_AUTH_F_AUTH (DH_KE getKey1 channel1 f1) (C getKey2 channel2 f2)).
-    iApply (F_AUTH_F_AUTH with "[$][$]"); [| |].
-    1,2 : simpl; repeat (rewrite andb_True; split); try set_solver; eauto using vunit_closed, vmult_closed, g_closed;
-          by apply is_closed_weaken_empty. 
-    by iApply (DH_KE_C_DH_real with "[$][$][$][$]"); eauto.
-  Qed.
     
   (* Verification of F_AUTH[C[DH_real]] ≤ F_AUTH[DH_KE] *)
   (*------------------------------------------------------------*)
-  Lemma F_AUTH_C_DH_real_FAUTH_DH_KE (f1 f2 : val) L X :
-    (*is_closed_expr ∅ f1 →
-    is_closed_expr ∅ f2 →*)
-    BREL f1 #()%V ≤ f2 #()%V <|LblAdv ++ L|> {{ λ v1 v2, ⌜ v1 = #()%V ∧ v2 = #()%V ⌝ }} -∗
-    BREL F_AUTH channel1 leakauth1 (C getKey1 channel1 DH_real f1) ≤ F_AUTH channel2 leakauth2 (DH_KE getKey2 channel2 f2) <|LblEnv ++ ([getKey1],[getKey2], X) :: L|> {{ λ v1 v2, ⌜ v1 = v2 ⌝ }}.
+  Lemma F_AUTH_C_DH_real_FAUTH_DH_KE (f1 f2 : val) L :
+    sem_val_typed f1 f2 (∀ᵣ θₕ, ((sem_ty_sum 𝟙 𝟙) -{ θₕ }-> (Option 𝔾)) -{ sem_row_union θₕ L }-> 𝟙)%T -∗
+    BREL F_AUTH channel1 leakauth1 (C channel1 DH_real f1) ≤ F_AUTH channel2 leakauth2 (DH_KE channel2 f2) <|LblEnv ++ (iLblSig_to_iLblThy L)|> {{ λ v1 v2, ⌜ v1 = v2 ⌝ }}.
   Proof using G inG0 inG1 inG2.
     iIntros "Hff".
     
@@ -1085,30 +1129,30 @@ Section handlee_verification.
     iMod dfrac_alloc as (γfracb) "Hfracb".                         
     iModIntro.
     
-    iApply (F_AUTH_F_AUTH with "[$][$]"); [| |].
-    
-    1,2 : simpl; repeat (rewrite andb_True; split); try set_solver; 
-      eauto using vunit_closed, vmult_closed, g_closed; by apply is_closed_weaken_empty. 
-    
-    by iApply (C_DH_real_DH_KE with "[$][$][$][$]"); eauto.
-  Qed.
-  
+  (*   iApply (F_AUTH_F_AUTH with "[$][$]"); [| |].
+       
+       1,2 : simpl; repeat (rewrite andb_True; split); try set_solver; 
+         eauto using vunit_closed, vmult_closed, g_closed; by apply is_closed_weaken_empty. 
+       
+       by iApply (C_DH_real_DH_KE with "[$][$][$][$]"); eauto.
+     Qed. *)
+  Admitted. 
   
   (* Move this to a new file *)
   (* Verification of DH_SIM[F_KE] ≤ C[DH_rand] *)
   (*--------------------------------------------------*)
   
-  Lemma DH_SIM_F_KE_C_DH_rand (f1 f2 : val) γtoka γtokb γfraca γfracb γautha γauthb L X :
-    let LblThy := LblAuthChannel γtoka atokN γtokb btokN γfraca γfracb γautha γauthb in
-    (*is_closed_expr ∅ f1 →
-    is_closed_expr ∅ f2 →*)
-    token γtoka -∗
-    token γtokb -∗
-    own γautha (to_dfrac_agree (DfracOwn 1) #()%V) -∗
-    own γauthb (to_dfrac_agree (DfracOwn 1) #()%V) -∗
-    BREL f1 #()%V ≤ f2 #()%V <|LblAdv ++ L|> {{ (λ v1 v2, ⌜v1 = #()%V ∧ v2 = #()%V⌝) }} -∗
-    BREL DH_SIM channel1 (F_KE getKey1 channel1 f1) ≤ C getKey2 channel2 DH_rand f2 <|([getKey1], [getKey2], X) :: LblThy ++ L|> {{ λ v1 v2, ⌜v1 = v2⌝ }}.
-  Proof using G inG0 inG1 inG2.
+  (* Lemma DH_SIM_F_KE_C_DH_rand (f1 f2 : val) γtoka γtokb γfraca γfracb γautha γauthb L X :
+       let LblThy := LblAuthChannel γtoka atokN γtokb btokN γfraca γfracb γautha γauthb in
+       (*is_closed_expr ∅ f1 →
+       is_closed_expr ∅ f2 →*)
+       token γtoka -∗
+       token γtokb -∗
+       own γautha (to_dfrac_agree (DfracOwn 1) #()%V) -∗
+       own γauthb (to_dfrac_agree (DfracOwn 1) #()%V) -∗
+       BREL f1 #()%V ≤ f2 #()%V <|LblAdv ++ L|> {{ (λ v1 v2, ⌜v1 = #()%V ∧ v2 = #()%V⌝) }} -∗
+       BREL DH_SIM channel1 (F_KE getKey1 channel1 f1) ≤ C getKey2 channel2 DH_rand f2 <|([getKey1], [getKey2], X) :: LblThy ++ L|> {{ λ v1 v2, ⌜v1 = v2⌝ }}.
+     Proof using G inG0 inG1 inG2. *)
    (*  iIntros (X' Hf1closed Hf2closed) "Htoka Htokb Ha Hb Hff".
        iApply rel_alloctape_l. iIntros (α) "!> Hα". rel_pures_l.
        iApply rel_alloctape_l. iIntros (β) "!> Hβ". rel_pures_l.
@@ -1406,22 +1450,22 @@ Section handlee_verification.
                   iApply (rel_exhaustion [_;_] [_] with "[$]"). iApply "IH". }
      Qed. *)
        
-    Admitted.
+   
 
   (* Verification of C[DH_rand] ≤ DH_SIM[F_KE] *)
   (*--------------------------------------------------*)  
 
-   Lemma C_DH_rand_DH_SIM_F_KE f1 f2 γtoka γtokb γfraca γfracb γautha γauthb L X :
-    let LblThy := LblAuthChannel γtoka atokN γtokb btokN γfraca γfracb γautha γauthb in
-    is_closed_expr ∅ f1 →
-    is_closed_expr ∅ f2 →
-    token γtoka -∗
-    token γtokb -∗
-    own γautha (to_dfrac_agree (DfracOwn 1) #()%V) -∗
-    own γauthb (to_dfrac_agree (DfracOwn 1) #()%V) -∗
-    BREL f1 ≤ f2 <|LblAdv ++ L|> {{ (λ v1 v2, ⌜v1 = #()%V ∧ v2 = #()%V⌝) }} -∗
-    BREL C getKey1 channel1 DH_rand f1 ≤ DH_SIM channel2 (F_KE getKey2 channel2 f2) <|([getKey1], [getKey2], X) :: LblThy ++ L|> {{ λ v1 v2, ⌜v1 = v2⌝ }}.
-   Proof using G inG0 inG1 inG2.
+   (* Lemma C_DH_rand_DH_SIM_F_KE f1 f2 γtoka γtokb γfraca γfracb γautha γauthb L X :
+       let LblThy := LblAuthChannel γtoka atokN γtokb btokN γfraca γfracb γautha γauthb in
+       is_closed_expr ∅ f1 →
+       is_closed_expr ∅ f2 →
+       token γtoka -∗
+       token γtokb -∗
+       own γautha (to_dfrac_agree (DfracOwn 1) #()%V) -∗
+       own γauthb (to_dfrac_agree (DfracOwn 1) #()%V) -∗
+       BREL f1 ≤ f2 <|LblAdv ++ L|> {{ (λ v1 v2, ⌜v1 = #()%V ∧ v2 = #()%V⌝) }} -∗
+       BREL C getKey1 channel1 DH_rand f1 ≤ DH_SIM channel2 (F_KE getKey2 channel2 f2) <|([getKey1], [getKey2], X) :: LblThy ++ L|> {{ λ v1 v2, ⌜v1 = v2⌝ }}.
+      Proof using G inG0 inG1 inG2. *)
    (*   iIntros (X' Hf1closed Hf2closed) "Htoka Htokb Ha Hb Hff".
         iApply rel_alloctape_r. iIntros (α) "Hα". rel_pures_r.
         rewrite subst_is_closed_empty; try done.
@@ -1724,60 +1768,59 @@ Section handlee_verification.
               (* First call is done. Can call getKey1 or getKey2 again. *)
               iApply (rel_exhaustion [_] [_;_] with "[$]"). iApply "IH". }
       Qed. *)
-   Admitted.
-
+ 
    
-  (* Verification of F_AUTH[DH_SIM[F_KE]] ≤ F_AUTH[C[DH_rand]] *)
-  (*------------------------------------------------------------*)
-  Lemma F_AUTH_DH_SIM_F_KE_FAUTH_C_DH_rand f1 f2 L X :
-    is_closed_expr ∅ f1 →
-    is_closed_expr ∅ f2 →
-    BREL f1 ≤ f2 <|LblAdv ++ L|> {{ λ v1 v2, ⌜ v1 = #()%V ∧ v2 = #()%V ⌝ }} -∗
-    BREL F_AUTH channel1 (DH_SIM channel1 (F_KE getKey1 channel1 f1)) ≤ F_AUTH channel2 (C getKey2 channel2 DH_rand f2) <|LblEnv ++ ([getKey1],[getKey2], X) :: L|> {{ λ v1 v2, ⌜ v1 = v2 ⌝ }}.
-  Proof using G inG0 inG1 inG2.
-    iIntros (Hf1closed Hf2closed) "Hff".
-    
-    iApply fupd_brel.
-    iMod token_alloc as (γtoka) "Htoka".
-    iMod token_alloc as (γtokb) "Htokb".
-    iMod (auth_alloc (#()%V)) as (γautha) "Hautha".
-    iMod (auth_alloc (#()%V)) as (γauthb) "Hauthb".
-    iMod dfrac_alloc as (γfraca) "Hfraca".
-    iMod dfrac_alloc as (γfracb) "Hfracb".                         
-    iModIntro.
-
-    iApply (F_AUTH_F_AUTH with "[$][$]"); [| |].
-    1,2 : simpl; repeat (rewrite andb_True; split); try set_solver; eauto using vunit_closed, vmult_closed, g_closed;
-          by apply is_closed_weaken_empty. 
-    by iApply (DH_SIM_F_KE_C_DH_rand with "[$][$][$][$]"); eauto.
-  Qed.
-    
-  (* Verification of F_AUTH[C[DH_rand]] ≤ F_AUTH[DH_SIM[F_KE]] *)
-  (*------------------------------------------------------------*)
-  Lemma F_AUTH_C_DH_rand_FAUTH_DH_SIM_F_KE f1 f2 L X :
-    is_closed_expr ∅ f1 →
-    is_closed_expr ∅ f2 →
-    BREL f1 ≤ f2 <|LblAdv ++ L|> {{ λ v1 v2, ⌜ v1 = #()%V ∧ v2 = #()%V ⌝ }} -∗
-    BREL F_AUTH channel1 (C getKey1 channel1 DH_rand f1) ≤ F_AUTH channel2 (DH_SIM channel2 (F_KE getKey2 channel2 f2)) <|LblEnv ++ ([getKey1],[getKey2], X) :: L|> {{ λ v1 v2, ⌜ v1 = v2 ⌝ }}.
-  Proof using G inG0 inG1 inG2.
-    iIntros (Hf1closed Hf2closed) "Hff".
-    
-    iApply fupd_brel.
-    iMod token_alloc as (γtoka) "Htoka".
-    iMod token_alloc as (γtokb) "Htokb".
-    iMod (auth_alloc (#()%V)) as (γautha) "Hautha".
-    iMod (auth_alloc (#()%V)) as (γauthb) "Hauthb".
-    iMod dfrac_alloc as (γfraca) "Hfraca".
-    iMod dfrac_alloc as (γfracb) "Hfracb".                         
-    iModIntro.
-
-    iApply (F_AUTH_F_AUTH with "[$][$]"); [| |].
-
-    1,2 : simpl; repeat (rewrite andb_True; split); try set_solver; 
-      eauto using vunit_closed, vmult_closed, g_closed; by apply is_closed_weaken_empty. 
-
-    by iApply (C_DH_rand_DH_SIM_F_KE with "[$][$][$][$]"); eauto.
-  Qed.
+  (* (* Verification of F_AUTH[DH_SIM[F_KE]] ≤ F_AUTH[C[DH_rand]] *)
+     (*------------------------------------------------------------*)
+     Lemma F_AUTH_DH_SIM_F_KE_FAUTH_C_DH_rand f1 f2 L X :
+       is_closed_expr ∅ f1 →
+       is_closed_expr ∅ f2 →
+       BREL f1 ≤ f2 <|LblAdv ++ L|> {{ λ v1 v2, ⌜ v1 = #()%V ∧ v2 = #()%V ⌝ }} -∗
+       BREL F_AUTH channel1 (DH_SIM channel1 (F_KE getKey1 channel1 f1)) ≤ F_AUTH channel2 (C getKey2 channel2 DH_rand f2) <|LblEnv ++ ([getKey1],[getKey2], X) :: L|> {{ λ v1 v2, ⌜ v1 = v2 ⌝ }}.
+     Proof using G inG0 inG1 inG2.
+       iIntros (Hf1closed Hf2closed) "Hff".
+       
+       iApply fupd_brel.
+       iMod token_alloc as (γtoka) "Htoka".
+       iMod token_alloc as (γtokb) "Htokb".
+       iMod (auth_alloc (#()%V)) as (γautha) "Hautha".
+       iMod (auth_alloc (#()%V)) as (γauthb) "Hauthb".
+       iMod dfrac_alloc as (γfraca) "Hfraca".
+       iMod dfrac_alloc as (γfracb) "Hfracb".                         
+       iModIntro.
+     
+       iApply (F_AUTH_F_AUTH with "[$][$]"); [| |].
+       1,2 : simpl; repeat (rewrite andb_True; split); try set_solver; eauto using vunit_closed, vmult_closed, g_closed;
+             by apply is_closed_weaken_empty. 
+       by iApply (DH_SIM_F_KE_C_DH_rand with "[$][$][$][$]"); eauto.
+     Qed.
+       
+     (* Verification of F_AUTH[C[DH_rand]] ≤ F_AUTH[DH_SIM[F_KE]] *)
+     (*------------------------------------------------------------*)
+     Lemma F_AUTH_C_DH_rand_FAUTH_DH_SIM_F_KE f1 f2 L X :
+       is_closed_expr ∅ f1 →
+       is_closed_expr ∅ f2 →
+       BREL f1 ≤ f2 <|LblAdv ++ L|> {{ λ v1 v2, ⌜ v1 = #()%V ∧ v2 = #()%V ⌝ }} -∗
+       BREL F_AUTH channel1 (C getKey1 channel1 DH_rand f1) ≤ F_AUTH channel2 (DH_SIM channel2 (F_KE getKey2 channel2 f2)) <|LblEnv ++ ([getKey1],[getKey2], X) :: L|> {{ λ v1 v2, ⌜ v1 = v2 ⌝ }}.
+     Proof using G inG0 inG1 inG2.
+       iIntros (Hf1closed Hf2closed) "Hff".
+       
+       iApply fupd_brel.
+       iMod token_alloc as (γtoka) "Htoka".
+       iMod token_alloc as (γtokb) "Htokb".
+       iMod (auth_alloc (#()%V)) as (γautha) "Hautha".
+       iMod (auth_alloc (#()%V)) as (γauthb) "Hauthb".
+       iMod dfrac_alloc as (γfraca) "Hfraca".
+       iMod dfrac_alloc as (γfracb) "Hfracb".                         
+       iModIntro.
+     
+       iApply (F_AUTH_F_AUTH with "[$][$]"); [| |].
+     
+       1,2 : simpl; repeat (rewrite andb_True; split); try set_solver; 
+         eauto using vunit_closed, vmult_closed, g_closed; by apply is_closed_weaken_empty. 
+     
+       by iApply (C_DH_rand_DH_SIM_F_KE with "[$][$][$][$]"); eauto.
+     Qed. *)
 
 End handlee_verification.
 
